Toy example: WPExcept.

Dijkstra.lean
@@ -11,3 +11,28 @@ import Dijkstra.Control.Monad.Dijkstra
 import Dijkstra.Control.Monad.Spec
 import Dijkstra.Control.Monad.Transformer
 
+universe u
+
+@[reducible]
+def WPExcept (ε : Type u) := ExceptT ε WPPure
+
+instance (ε : Type u) : Monad (WPExcept ε) :=
+  inferInstanceAs (Monad (ExceptT ε WPPure))
+
+instance (ε : Type u) : SpecMonad (WPExcept ε) where
+  rel {α} x y := ∀ (p : Except ε α → Prop), y.predT p → x.predT p
+  rel_pure a p := by dsimp; exact id
+  rel_bind {α} {β} {x} {y} f g hxy hfg p := by
+    dsimp [bind] at *
+    dsimp [ExceptT.bind, ExceptT.mk]
+    apply SpecMonad.toMonadRel.rel_bind (m:=WPPure) (n:=WPPure) hxy
+    intro a
+    cases a
+    case a.error e =>
+      dsimp [ExceptT.bindCont]
+      exact SpecMonad.toMonadRel.rel_pure (m:=WPPure) (n:=WPPure) _
+    case a.ok a =>
+      dsimp [ExceptT.bindCont]
+      exact hfg a
+
+example (ε : Type u) (α : Type _) : WPPure α → WPExcept ε α := monadLift
